pass

Iris/Iris/Algebra/Functions.lean
@@ -23,13 +23,29 @@ composition, and update laws.
 
 @[rocq_alias discrete_fun_insert]
 def discreteFunInsert {ι : Type _} [DecidableEq ι] {β : ι → Type _}
-    [∀ i, OFE (β i)] (x : ι) (y : β x) (f : (a : ι) → β a) : (a : ι) → β a :=
+    (x : ι) (y : β x) (f : (a : ι) → β a) : (a : ι) → β a :=
   fun x' => if h : x = x' then h ▸ y else f x'
 
 @[rocq_alias discrete_fun_singleton]
 def discreteFunSingleton {ι : Type _} [DecidableEq ι] {β : ι → Type _}
     [∀ i, UCMRA (β i)] (x : ι) (y : β x) : (a : ι) → β a :=
   discreteFunInsert x y fun _ => unit
+
+section insert
+
+variable {ι : Type _} [DecidableEq ι] {β : ι → Type _}
+
+@[rocq_alias discrete_fun_lookup_insert, simp]
+theorem discreteFunInsert_self (f : (a : ι) → β a) (x : ι) (y : β x) :
+    discreteFunInsert x y f x = y := by
+  simp [discreteFunInsert]
+
+@[rocq_alias discrete_fun_lookup_insert_ne, simp]
+theorem discreteFunInsert_of_ne (f : (a : ι) → β a) (x x' : ι)
+    (y : β x) (h : x ≠ x') : discreteFunInsert x y f x' = f x' := by
+  simp [discreteFunInsert, h]
+
+end insert
 
 section OFE
 
@@ -40,48 +56,44 @@ instance instDiscreteFunOfeDiscrete [∀ i, OFE.Discrete (β i)] :
     OFE.Discrete ((i : ι) → β i) where
   discrete_0 h _ i := (OFE.Discrete.discrete_0 (h i)).dist
 
-private instance instDiscreteFunDiscreteE (f : (a : ι) → β a)
-    [∀ i, DiscreteE (f i)] : DiscreteE f where
-  discrete h _ i := (DiscreteE.discrete (h i)).dist
+omit [DecidableEq ι] in
+/-- Not an instance, cycle with `discreteE_apply`. -/
+theorem discreteE_pi {f : (a : ι) → β a} (hf : ∀ i, DiscreteE (f i)) : DiscreteE f where
+  discrete h _ i := ((hf i).discrete (h i)).dist
 
 @[rocq_alias discrete_fun_insert_ne]
 instance instDiscreteFunInsertNonExpansive (x : ι) :
     NonExpansive₂ (discreteFunInsert (β := β) x) where
   ne {n y₁ y₂} hy {f₁ f₂} hf x' := by
-    simp only [discreteFunInsert]
-    split <;> subst_vars <;> first | exact hy | exact hf x'
+    by_cases h : x = x'
+    · subst h
+      simpa using hy
+    · rw [discreteFunInsert_of_ne (h := h) .., discreteFunInsert_of_ne (h := h) ..]
+      exact hf x'
 
 #rocq_ignore discrete_fun_insert_proper "Use the NonExpansive instance instead."
 
-@[rocq_alias discrete_fun_lookup_insert]
-theorem discrete_fun_lookup_insert (f : (a : ι) → β a) (x : ι) (y : β x) :
-    discreteFunInsert x y f x = y := by
-  simp [discreteFunInsert]
-
-@[rocq_alias discrete_fun_lookup_insert_ne]
-theorem discrete_fun_lookup_insert_ne (f : (a : ι) → β a) (x x' : ι)
-    (y : β x) (h : x ≠ x') : discreteFunInsert x y f x' = f x' := by
-  simp [discreteFunInsert, h]
-
-private instance discreteE_apply (f : (a : ι) → β a) [DiscreteE f] (x : ι) :
+/-- Not an instance, cycle with `discreteE_pi`. -/
+theorem discreteE_apply {f : (a : ι) → β a} (hf : DiscreteE f) (x : ι) :
     DiscreteE (f x) where
   discrete {y} h n := by
-    have hfun : f ≡{0}≡ discreteFunInsert x y f := by
-      intro x'
+    have hfun : f ≡{0}≡ discreteFunInsert x y f := fun x' => by
       by_cases hxx' : x = x'
-      · subst x'
-        simpa [discrete_fun_lookup_insert] using h
-      · rw [discrete_fun_lookup_insert_ne (h := hxx') ..]
-    simpa only [discrete_fun_lookup_insert] using DiscreteE.discrete hfun n x
+      · subst hxx'
+        simpa using h
+      · rw [discreteFunInsert_of_ne (h := hxx') ..]
+    simpa only [discreteFunInsert_self] using hf.discrete hfun n x
 
 @[rocq_alias discrete_fun_insert_discrete]
 instance instDiscreteFunInsertDiscrete (f : (a : ι) → β a) (x : ι) (y : β x)
-    [DiscreteE f] [DiscreteE y] : DiscreteE (discreteFunInsert x y f) := by
-  letI : ∀ i, DiscreteE (discreteFunInsert x y f i) := fun x' => by
-    simp only [discreteFunInsert]
-    split <;> subst_vars <;> infer_instance
-  infer_instance
-
+    [DiscreteE f] [DiscreteE y] : DiscreteE (discreteFunInsert x y f) :=
+  discreteE_pi fun x' => by
+    by_cases h : x = x'
+    · subst h
+      rw [discreteFunInsert_self]
+      infer_instance
+    · rw [discreteFunInsert_of_ne (h := h) ..]
+      exact discreteE_apply ‹DiscreteE f› x'
 
 end OFE
 
@@ -101,125 +113,144 @@ instance instDiscreteFunSingletonNonExpansive (x : ι) :
 
 #rocq_ignore discrete_fun_singleton_proper "Use NonExpansive instance instead."
 
-@[rocq_alias discrete_fun_lookup_singleton]
-theorem discrete_fun_lookup_singleton {x : ι} (y : β x) :
-    discreteFunSingleton x y x = y := discrete_fun_lookup_insert ..
+@[rocq_alias discrete_fun_lookup_singleton, simp]
+theorem discreteFunSingleton_self {x : ι} (y : β x) :
+    discreteFunSingleton x y x = y := discreteFunInsert_self ..
 
-@[rocq_alias discrete_fun_lookup_singleton_ne]
-theorem discrete_fun_lookup_singleton_ne {x x' : ι} (y : β x) (h : x ≠ x') :
+@[rocq_alias discrete_fun_lookup_singleton_ne, simp]
+theorem discreteFunSingleton_of_ne {x x' : ι} (y : β x) (h : x ≠ x') :
     discreteFunSingleton x y x' = unit :=
-  discrete_fun_lookup_insert_ne (h := h) ..
+  discreteFunInsert_of_ne (h := h) ..
 
 @[rocq_alias discrete_fun_singleton_discrete]
 instance instDiscreteFunSingletonDiscrete {x : ι} (y : β x)
     [∀ i, DiscreteE (unit : β i)] [DiscreteE y] :
     DiscreteE (discreteFunSingleton x y) :=
+  haveI : DiscreteE fun i : ι => (unit : β i) := discreteE_pi fun _ => inferInstance
   instDiscreteFunInsertDiscrete (fun _ => unit) x y
 
 @[rocq_alias discrete_fun_singleton_validN]
-theorem discrete_fun_singleton_validN_iff (n : Nat) {x : ι} (y : β x) :
+theorem discreteFunSingleton_validN_iff (n : Nat) {x : ι} (y : β x) :
     ✓{n} discreteFunSingleton x y ↔ ✓{n} y := by
   constructor
-  · exact fun h => discrete_fun_lookup_singleton y ▸ h x
+  · exact fun h => discreteFunSingleton_self y ▸ h x
   · intro hy x'
-    simp only [discreteFunSingleton, discreteFunInsert]
-    split <;> subst_vars <;> first | exact hy | exact unit_validN
+    by_cases h : x = x'
+    · subst h
+      rw [discreteFunSingleton_self]
+      exact hy
+    · rw [discreteFunSingleton_of_ne y h]
+      exact unit_validN
 
 @[rocq_alias discrete_fun_singleton_valid]
-theorem discrete_fun_singleton_valid_iff {x : ι} (y : β x) :
+theorem discreteFunSingleton_valid_iff {x : ι} (y : β x) :
     ✓ discreteFunSingleton x y ↔ ✓ y := by
   rw [valid_iff_validN, valid_iff_validN]
-  exact forall_congr' fun n => discrete_fun_singleton_validN_iff ..
+  exact forall_congr' fun n => discreteFunSingleton_validN_iff ..
 
 @[rocq_alias discrete_fun_singleton_unit]
-theorem discrete_fun_singleton_unit_equiv (x : ι) :
+theorem discreteFunSingleton_unit_eqv (x : ι) :
     discreteFunSingleton x (unit : β x) ≡ (unit : (a : ι) → β a) := by
   intro n x'
-  simp only [discreteFunSingleton, discreteFunInsert]
-  split <;> subst_vars <;> rfl
+  by_cases h : x = x'
+  · subst h
+    rw [discreteFunSingleton_self]
+    exact .rfl
+  · rw [discreteFunSingleton_of_ne _ h]
+    exact .rfl
 
 @[rocq_alias discrete_fun_singleton_core]
-theorem discrete_fun_singleton_core_equiv {x : ι} (y : β x) :
+theorem discreteFunSingleton_core_eqv {x : ι} (y : β x) :
     core (discreteFunSingleton x y) ≡ discreteFunSingleton x (core y) := by
   intro n x'
-  simp only [core, CMRA.pcore, Option.getD_some, discreteFunSingleton, discreteFunInsert]
-  split <;> subst_vars <;> first | rfl | exact (core_eqv_self unit).dist
+  simp only [core, CMRA.pcore, Option.getD_some]
+  by_cases h : x = x'
+  · subst h
+    rw [discreteFunSingleton_self, discreteFunSingleton_self]
+  · rw [discreteFunSingleton_of_ne y h, discreteFunSingleton_of_ne _ h]
+    exact (core_eqv_self unit).dist
 
 @[rocq_alias discrete_fun_singleton_core_id]
 instance instDiscreteFunSingletonCoreId (x : ι) (y : β x) [CoreId y] :
     CoreId (discreteFunSingleton x y) :=
-  coreId_iff_core_eqv_self.mpr <| (discrete_fun_singleton_core_equiv y).trans
+  coreId_iff_core_eqv_self.mpr <| (discreteFunSingleton_core_eqv y).trans
     <| NonExpansive.eqv (core_eqv_self y)
 
 @[rocq_alias discrete_fun_singleton_op]
-theorem discrete_fun_singleton_op_equiv {x : ι} (y₁ y₂ : β x) :
+theorem discreteFunSingleton_op_eqv {x : ι} (y₁ y₂ : β x) :
     discreteFunSingleton x y₁ • discreteFunSingleton x y₂ ≡
       discreteFunSingleton x (y₁ • y₂) := by
   intro n x'
-  simp only [CMRA.op, discreteFunSingleton, discreteFunInsert]
-  split <;> subst_vars <;> first | rfl | exact unit_left_id.dist
+  simp only [CMRA.op]
+  by_cases h : x = x'
+  · subst h
+    rw [discreteFunSingleton_self, discreteFunSingleton_self, discreteFunSingleton_self]
+  · rw [discreteFunSingleton_of_ne y₁ h, discreteFunSingleton_of_ne y₂ h,
+      discreteFunSingleton_of_ne _ h]
+    exact unit_left_id.dist
 
 @[rocq_alias discrete_fun_insert_updateP]
-theorem discrete_fun_insert_update_pred {x : ι} {P : β x → Prop} {Q : ((a : ι) → β a) → Prop}
-    {g : (a : ι) → β a} {y₁ : β x} (hy : y₁ ~~>: P) (hQ : ∀ y₂, P y₂ → Q (discreteFunInsert x y₂ g)) :
+theorem discreteFunInsert_updateP {x : ι} {P : β x → Prop} {Q : ((a : ι) → β a) → Prop}
+    {g : (a : ι) → β a} {y₁ : β x} (hy : y₁ ~~>: P)
+    (hQ : ∀ y₂, P y₂ → Q (discreteFunInsert x y₂ g)) :
     discreteFunInsert x y₁ g ~~>: Q := by
   refine UpdateP.total.mpr fun n gf hgf => ?_
   have hgf_at (a : ι) : ✓{n} discreteFunInsert x y₁ g a • gf a := hgf a
-  obtain ⟨y₂, hy₂, hvalid⟩ :=
-    hy n (some (gf x)) (by
-      simpa only [CMRA.op?, discrete_fun_lookup_insert] using hgf_at x)
+  obtain ⟨y₂, hy₂, hvalid⟩ := hy n (some (gf x))
+    (by simpa only [CMRA.op?, discreteFunInsert_self] using hgf_at x)
   refine ⟨discreteFunInsert x y₂ g, hQ y₂ hy₂, fun x' => ?_⟩
   simp only [CMRA.op]
   by_cases hx'x : x' = x
   · subst x'
-    simpa only [CMRA.op?, discrete_fun_lookup_insert]
-  · simpa only [discrete_fun_lookup_insert_ne (h := Ne.symm hx'x) ..] using hgf_at x'
+    simpa only [CMRA.op?, discreteFunInsert_self]
+  · simpa only [discreteFunInsert_of_ne (h := Ne.symm hx'x) ..] using hgf_at x'
 
 @[rocq_alias discrete_fun_insert_updateP']
-theorem discrete_fun_insert_update_pred_witness {x : ι} {P : β x → Prop} (g : (a : ι) → β a)
+theorem discreteFunInsert_updateP' {x : ι} {P : β x → Prop} (g : (a : ι) → β a)
     {y₁ : β x} (hy : y₁ ~~>: P) :
     discreteFunInsert x y₁ g ~~>: fun g' => ∃ y₂, g' = discreteFunInsert x y₂ g ∧ P y₂ :=
-  discrete_fun_insert_update_pred hy fun y₂ hy₂ => ⟨y₂, rfl, hy₂⟩
+  discreteFunInsert_updateP hy fun y₂ hy₂ => ⟨y₂, rfl, hy₂⟩
 
 @[rocq_alias discrete_fun_insert_update]
-theorem discrete_fun_insert_update (g : (a : ι) → β a) {x : ι} {y₁ y₂ : β x} (hy : y₁ ~~> y₂) :
+theorem discreteFunInsert_update (g : (a : ι) → β a) {x : ι} {y₁ y₂ : β x} (hy : y₁ ~~> y₂) :
     discreteFunInsert x y₁ g ~~> discreteFunInsert x y₂ g :=
-  Update.of_updateP <| discrete_fun_insert_update_pred (UpdateP.of_update hy) fun _ hy₂ => hy₂ ▸ rfl
+  Update.of_updateP <| discreteFunInsert_updateP (UpdateP.of_update hy) fun _ hy₂ => hy₂ ▸ rfl
 
 @[rocq_alias discrete_fun_singleton_updateP]
-theorem discrete_fun_singleton_update_pred {x : ι} {P : β x → Prop} (Q : ((a : ι) → β a) → Prop)
+theorem discreteFunSingleton_updateP {x : ι} {P : β x → Prop} (Q : ((a : ι) → β a) → Prop)
     {y₁ : β x} (hy : y₁ ~~>: P) (hQ : ∀ y₂, P y₂ → Q (discreteFunSingleton x y₂)) :
     discreteFunSingleton x y₁ ~~>: Q :=
-  discrete_fun_insert_update_pred hy hQ
+  discreteFunInsert_updateP hy hQ
 
 @[rocq_alias discrete_fun_singleton_updateP']
-theorem discrete_fun_singleton_update_pred_witness {x : ι} {P : β x → Prop}
+theorem discreteFunSingleton_updateP' {x : ι} {P : β x → Prop}
     {y₁ : β x} (hy : y₁ ~~>: P) :
     discreteFunSingleton x y₁ ~~>: fun g => ∃ y₂, g = discreteFunSingleton x y₂ ∧ P y₂ :=
-  discrete_fun_singleton_update_pred _ hy fun y₂ hy₂ => ⟨y₂, rfl, hy₂⟩
+  discreteFunSingleton_updateP _ hy fun y₂ hy₂ => ⟨y₂, rfl, hy₂⟩
 
 @[rocq_alias discrete_fun_singleton_update]
-theorem discrete_fun_singleton_update {x : ι} {y₁ y₂ : β x} (hy : y₁ ~~> y₂) :
+theorem discreteFunSingleton_update {x : ι} {y₁ y₂ : β x} (hy : y₁ ~~> y₂) :
     discreteFunSingleton x y₁ ~~> discreteFunSingleton x y₂ :=
-  discrete_fun_insert_update _ hy
+  discreteFunInsert_update _ hy
 
 @[rocq_alias discrete_fun_singleton_updateP_empty]
-theorem discrete_fun_singleton_update_p_unit {x : ι} {P : β x → Prop} {Q : ((a : ι) → β a) → Prop}
-    (hy : unit ~~>: P) (hQ : ∀ y₂, P y₂ → Q (discreteFunSingleton x y₂)) : unit ~~>: Q :=
-  UpdateP.equiv_left (discrete_fun_singleton_unit_equiv x) <|
-    discrete_fun_singleton_update_pred Q hy hQ
+theorem discreteFunSingleton_updateP_unit {x : ι} {P : β x → Prop}
+    {Q : ((a : ι) → β a) → Prop} (hy : unit ~~>: P)
+    (hQ : ∀ y₂, P y₂ → Q (discreteFunSingleton x y₂)) : unit ~~>: Q :=
+  UpdateP.equiv_left (discreteFunSingleton_unit_eqv x) <|
+    discreteFunSingleton_updateP Q hy hQ
 
 @[rocq_alias discrete_fun_singleton_updateP_empty']
-theorem discrete_fun_singleton_update_p_unit_witness {x : ι} {P : β x → Prop}
+theorem discreteFunSingleton_updateP_unit' {x : ι} {P : β x → Prop}
     (hy : (unit : β x) ~~>: P) :
     unit ~~>: fun g => ∃ y₂, g = discreteFunSingleton x y₂ ∧ P y₂ :=
-  discrete_fun_singleton_update_p_unit hy fun y₂ hy₂ => ⟨y₂, rfl, hy₂⟩
+  discreteFunSingleton_updateP_unit hy fun y₂ hy₂ => ⟨y₂, rfl, hy₂⟩
 
 @[rocq_alias discrete_fun_singleton_update_empty]
-theorem discrete_fun_singleton_update_unit {x : ι} {y : β x} (hy : unit ~~> y) :
+theorem discreteFunSingleton_update_unit {x : ι} {y : β x} (hy : unit ~~> y) :
     unit ~~> discreteFunSingleton x y :=
   Update.of_updateP <|
-    discrete_fun_singleton_update_p_unit (UpdateP.of_update hy) <| fun _ hz => hz ▸ rfl
+    discreteFunSingleton_updateP_unit (UpdateP.of_update hy) <| fun _ hz => hz ▸ rfl
 
 end CMRA
 
@@ -228,26 +259,22 @@ section CMRA
 variable {ι : Type _} {β : ι → Type _} [∀ i, UCMRA (β i)]
 
 @[rocq_alias discrete_fun_updateP]
-theorem discrete_fun_update_pred {f : (a : ι) → β a} {P : (a : ι) → β a → Prop} {Q : ((a : ι) → β a) → Prop}
-    (hf : ∀ a, f a ~~>: P a) (hQ : ∀ f', (∀ a, P a (f' a)) → Q f') : f ~~>: Q := by
+theorem discreteFun_updateP {f : (a : ι) → β a} {P : (a : ι) → β a → Prop}
+    {Q : ((a : ι) → β a) → Prop} (hf : ∀ a, f a ~~>: P a)
+    (hQ : ∀ f', (∀ a, P a (f' a)) → Q f') : f ~~>: Q := by
   refine UpdateP.total.mpr fun n g hfg => ?_
-  have hchoice : ∀ a, ∃ y, P a y ∧ ✓{n} y • g a := fun a =>
-    hf a n (some (g a)) (hfg a)
-  let f' : (a : ι) → β a := fun a => Classical.choose (hchoice a)
-  refine ⟨f', hQ f' fun a => (Classical.choose_spec (hchoice a)).1,
-    fun a => (Classical.choose_spec (hchoice a)).2⟩
+  obtain ⟨f', hf'⟩ := Classical.axiomOfChoice fun a => hf a n (some (g a)) (hfg a)
+  exact ⟨f', hQ f' fun a => (hf' a).1, fun a => (hf' a).2⟩
 
 @[rocq_alias discrete_fun_updateP']
-theorem discrete_fun_update_pred_pointwise {f : (a : ι) → β a} {P : (a : ι) → β a → Prop}
+theorem discreteFun_updateP' {f : (a : ι) → β a} {P : (a : ι) → β a → Prop}
     (hf : ∀ a, f a ~~>: P a) : f ~~>: fun f' => ∀ a, P a (f' a) :=
-  discrete_fun_update_pred hf fun _ h => h
+  discreteFun_updateP hf fun _ h => h
 
 @[rocq_alias discrete_fun_update]
-theorem discrete_fun_update {f g : (a : ι) → β a} (hfg : ∀ a, f a ~~> g a) :
-    f ~~> g := fun n mh v a =>
-  match mh with
-  | none => hfg a n none (v a)
-  | some h => hfg a n (some (h a)) (v a)
+theorem discreteFun_update {f g : (a : ι) → β a} (hfg : ∀ a, f a ~~> g a) : f ~~> g :=
+  Update.of_updateP <| discreteFun_updateP (fun a => UpdateP.of_update (hfg a))
+    fun _ h => funext h
 
 end CMRA
 
